cedar-lean/Cedar/Thm/Translation/PolicyToExpr.lean
@@ -1,0 +1,24 @@
+import Cedar.Spec
+import Cedar.Spec.Cst
+import Cedar.Spec.CstSemantics
+import Cedar.Spec.CstToAst
+import Cedar.Thm.Translation.Aux
+import Cedar.Thm.Data.List.Lemmas
+
+namespace Cedar.Thm
+
+open Cedar.Data
+open Cedar.Spec
+
+
+theorem policy_to_expr_agrees (cp : Cst.Policy) (ap : Policy)
+  (ce : Cst.Expr) (ae : Expr) :
+  cp.toPolicy? = some ap →
+  cp.toExpr = ce →
+  ce.toAExpr? = some ae →
+  ap.toExpr = ae := by
+
+  intro hap hce hae
+  obtain ⟨p⟩ := cp
+  obtain ⟨eff, vars, conds⟩ := p
+  sorry
